thys/Transition_Systems_and_Automata/Automata/NBA/NGBA.thy
@@ -13,7 +13,8 @@ begin
   global_interpretation ngba: automaton ngba alphabet initial transition accepting
     defines path = ngba.path and run = ngba.run and reachable = ngba.reachable and nodes = ngba.nodes
     by unfold_locales auto
-  global_interpretation ngba: automaton_trace ngba alphabet initial transition accepting "gen infs"
+  global_interpretation ngba: automaton_trace ngba alphabet initial transition accepting
+    "\<lambda> P w r p. gen infs P (ngba.trace (w ||| r) p)"
     defines language = ngba.language
     by standard
 
